src/named/MultiCompilers.v
@@ -1,0 +1,1158 @@
+Set Implicit Arguments.
+Set Bullet Behavior "Strict Subproofs".
+
+Require Import String List.
+Import ListNotations.
+Open Scope string.
+Open Scope list.
+From Utils Require Import Utils.
+From Named Require Import Core AllConstructors.
+Import Core.Notations.
+(*TODO: rename this to compiler proofs and have a separate export-only file?*)
+Require Export MultiCompilerDefs.
+
+
+Lemma flat_map_all_empty {A B} (f : A -> list B) l
+  : (forall x, f x = []) ->
+    flat_map f l = [].
+Proof.
+  induction l; basic_goal_prep; basic_utils_firstorder_crush.
+  rewrite H, H0.
+  reflexivity.
+Qed.
+
+Lemma compile_ctx_empty cmp
+  : compile_ctx cmp [] = [].
+Proof.
+  unfold compile_ctx.
+  rewrite flat_map_all_empty; auto.
+Qed.  
+Hint Rewrite compile_ctx_empty : lang_core.
+
+
+Lemma map_flat_map {A B C} (f : B -> C) (g : A -> list B) l
+  : map f (flat_map g l) = flat_map (fun x => map f (g x)) l.
+Admitted.
+
+
+Lemma named_map_fst_eq {A B}
+  : forall (f : A -> B) (l1 : named_list A), map fst (named_map f l1) = map fst l1.
+Admitted.
+
+
+Lemma flat_map_ext {A B} (f g : A -> list B) l
+  : (forall x, f x = g x) -> (flat_map f l) = flat_map g l.
+Admitted.
+
+Lemma flat_map_f_cons {A B} f (g : A -> list B) l x b
+  : In x l -> b = f x -> In b (flat_map (fun x => (f x)::(g x)) l).
+Admitted.
+
+
+
+
+Lemma fresh_compile_ctx_cons cname x l0 n l s c 
+  : fresh (cname :: x) (compile_ctx (l0, n) ((l, s) :: c)) <->
+      (fresh (cname :: x) (map (fun '(n', t) => (cname :: n', compile_sort (l0, n) cname t)) c)
+      /\ fresh (cname :: x) (compile_ctx (l0, n) c)).
+Admitted.
+Hint Rewrite fresh_compile_ctx_cons : lang_core.
+
+Lemma fresh_compile_ctx x cmp c cname
+  : In cname (fst cmp) ->
+    fresh (cname::x) (compile_ctx cmp c) <-> fresh x c.
+Proof.
+  induction c; basic_goal_prep;
+    basic_core_firstorder_crush.
+  {
+    apply H0.
+    rewrite map_map.
+    erewrite map_ext.
+    2:{
+      instantiate (1:= fun p => cname::(fst p)).
+      intros; destruct a; reflexivity.
+    }
+    simpl.
+      auto. (*
+      intro a.
+      inst
+      destruct a.
+      
+      reflexivity.
+      simpl. reflexivity.
+    simpl.
+    rewrite map_flat_map.
+    erewrite flat_map_ext.
+    2: intros; apply map_map.
+    simpl.
+    eapply flat_map_f_cons; eauto.
+  }
+      let __ := match constr:(Set) with _ =>
+          syntactic_unify_deltavar x y end in
+  {
+    apply fresh_compile_ctx_cons_tl in H0.
+    auto.
+  }
+  {
+    
+    rewrite fresh_cons in H0.
+    basic_core_crush.
+    destruct H0. basic_core_crush.
+    apply H1.
+
+    }
+    
+    cbv [compile_ctx fst named_map].
+    simpl.
+    unfold In.*)
+Admitted.
+(*
+Hint Rewrite fresh_compile_ctx : lang_core.*)
+
+(*
+
+Lemma all_fresh_compile_ctx cmp c
+  : all_fresh (compile_ctx cmp c) <-> all_fresh c.
+Proof.
+  induction c; basic_goal_prep;
+    basic_core_crush.
+Qed.
+Hint Rewrite all_fresh_compile_ctx : lang_core.
+
+*)
+
+Lemma fresh_lang_fresh_cmp cmp_pre lt cmp l n
+  : preserving_compiler_ext cmp_pre lt cmp l ->
+    fresh n l -> fresh n cmp.
+Proof.
+  induction 1; basic_goal_prep;
+    basic_core_crush.
+Qed.
+Hint Resolve fresh_lang_fresh_cmp : lang_core.
+
+
+Lemma all_fresh_compiler lt names cmp l
+  : preserving_compiler_ext (names,[]) lt cmp l ->
+    all_fresh l ->
+    all_fresh cmp.
+Proof.
+  induction 1;
+    basic_goal_prep;
+    basic_core_crush.
+Qed.
+Hint Resolve all_fresh_compiler : lang_core.
+
+(*TODO: move to source*)
+Arguments eqb {A}%type_scope {Eqb} !_ !_ /.
+
+(*TODO: move to utils*)
+Lemma flat_map_funext {A B} (f g : A ->  list B) l
+  : (forall x, In x l -> f x = g x) ->
+    flat_map f l = flat_map g l.
+Proof.
+  intros; induction l; basic_goal_prep; basic_utils_crush.
+  rewrite H, IHl; auto.
+Qed.
+
+Lemma compile_strengthen_term cmp n cc e cname
+  : fresh n (snd cmp) ->
+    all_fresh (snd cmp) ->
+    all_constructors (fun n => In n (map fst (snd cmp))) e ->
+    compile (extend_cmp [(n,cc)] cmp) cname e = compile cmp cname e.
+Proof.
+  revert cname.
+  induction e; basic_goal_prep; basic_core_crush.
+  my_case Heq (eqb n0 n); basic_goal_prep;
+    basic_core_crush.
+  case_match; basic_goal_prep;
+      basic_core_crush.
+  case_match; basic_goal_prep;
+    basic_core_crush.
+  f_equal.
+  f_equal.
+  apply flat_map_funext.
+  intros x Inx.
+  apply map_ext_in.
+  intros a Ina.
+  pose proof (in_all _ _ H Ina).
+  simpl in *.
+  apply H2; auto.
+  eapply in_all; eauto.
+Qed.
+Hint Rewrite compile_strengthen_term : lang_core.
+
+
+Lemma compile_args_cons_eq l n1 n2 a e
+  : (forall cname, In cname l -> compile (l, n1) cname a = compile (l, n2) cname a) ->
+    compile_args (l, n1) e = compile_args (l, n2) e ->
+    compile_args (l, n1) (a :: e) = compile_args (l, n2) (a :: e).
+Proof.
+  unfold compile_args.
+  induction l; basic_goal_prep; basic_core_crush.
+  f_equal.
+  {
+    clear IHl.
+    append_eq_same_len
+Qed.
+
+Lemma compile_strengthen_args cmp n cc e
+  : fresh n (snd cmp) ->
+    all_fresh (snd cmp) ->
+    all (all_constructors (fun n => In n (map fst (snd cmp)))) e ->
+    compile_args (extend_cmp [(n,cc)] cmp) e = compile_args cmp e.
+Proof.
+  induction e; basic_goal_prep; basic_core_crush.
+  apply compile_args_cons_eq.
+  basic_goal_prep; basic_core_crush.
+  unfold compile_args.
+  simpl.
+Qed.
+Hint Rewrite compile_strengthen_args : lang_core.
+
+Lemma compile_strengthen_sort cmp n cc e
+  : fresh n cmp ->
+    all_fresh cmp ->
+    all_constructors_sort (fun n => In n (map fst cmp)) e ->
+    compile_sort ((n,cc)::cmp) e = compile_sort cmp e.
+Proof.
+  destruct e; basic_goal_prep; basic_core_crush.
+  my_case Heq (eqb v n); basic_goal_prep;
+    basic_core_crush.
+  case_match; basic_goal_prep;
+      basic_core_crush.
+  case_match; basic_goal_prep;
+    basic_core_crush.
+  f_equal.
+  f_equal.
+  apply compile_strengthen_args; assumption.
+Qed.
+Hint Rewrite compile_strengthen_sort : lang_core.
+
+
+Lemma compile_strengthen_ctx cmp n cc c
+  : fresh n cmp ->
+    all_fresh cmp ->
+    all (fun '(_,t) => all_constructors_sort (fun n => In n (map fst cmp)) t) c ->
+    compile_ctx ((n,cc)::cmp) c = compile_ctx cmp c.
+Proof.
+  induction c; basic_goal_prep; f_equal; basic_core_crush.
+Qed.
+Hint Rewrite compile_strengthen_ctx : lang_core.
+
+
+Lemma sort_name_in_cmp cmp_pre tgt cmp src c' args n
+  : preserving_compiler_ext cmp_pre tgt cmp src ->
+    In (n, sort_rule c' args) src ->
+    In n (map fst cmp).
+Proof.
+  induction 1;basic_goal_prep;
+    with_rule_in_wf_crush.
+Qed.
+Local Hint Resolve sort_name_in_cmp : lang_core.
+
+Lemma term_name_in_cmp cmp_pre tgt cmp src c' args t n
+  : preserving_compiler_ext cmp_pre tgt cmp src ->
+    In (n, term_rule c' args t) src ->
+    In n (map fst cmp).
+Proof.
+  induction 1;basic_goal_prep;
+    with_rule_in_wf_crush.
+Qed.
+Local Hint Resolve term_name_in_cmp : lang_core.
+                   
+Local Lemma all_constructors_from_wf tgt cmp src
+  : preserving_compiler_ext [] tgt cmp src ->
+    (forall c t,
+        wf_sort src c t ->
+        all_constructors_sort (fun n0 : V => In n0 (map fst cmp)) t)
+    /\ (forall c e t,
+           wf_term src c e t ->
+           all_constructors (fun n0 : V => In n0 (map fst cmp)) e)
+    /\ (forall c s c',
+           wf_args src c s c' ->
+           all (all_constructors (fun n0 : V => In n0 (map fst cmp))) s).
+Proof using.
+  intros; apply wf_judge_ind; basic_goal_prep;
+    with_rule_in_wf_crush.
+Qed.
+
+Definition all_constructors_sort_from_wf tgt cmp src (pr : preserving_compiler_ext [] tgt cmp src)
+  := proj1 (all_constructors_from_wf pr).
+Hint Resolve all_constructors_sort_from_wf : lang_core.
+
+Definition all_constructors_term_from_wf tgt cmp src (pr : preserving_compiler_ext [] tgt cmp src)
+  := proj1 (proj2 (all_constructors_from_wf pr)).
+Hint Resolve all_constructors_term_from_wf : lang_core.
+
+Definition all_constructors_args_from_wf tgt cmp src (pr : preserving_compiler_ext [] tgt cmp src)
+  := proj2 (proj2 (all_constructors_from_wf pr)).
+Hint Resolve all_constructors_args_from_wf : lang_core.
+
+Lemma all_constructors_ctx_from_wf tgt cmp src c
+  : preserving_compiler_ext [] tgt cmp src ->
+    wf_ctx src c ->
+    all_constructors_ctx (fun n0 : V => In n0 (map fst cmp)) c.
+Proof.
+  induction 2; basic_goal_prep;
+    with_rule_in_wf_crush.
+Qed.
+Hint Resolve all_constructors_ctx_from_wf : lang_core.
+
+
+(*TODO: think about whether this should be generalized*)
+Lemma inductive_implies_semantic_sort_axiom ls lt cmp name c t1 t2
+  : wf_lang lt -> preserving_compiler_ext [] lt cmp ls -> wf_lang ls ->
+    In (name, sort_eq_rule c t1 t2) ls ->
+    eq_sort lt (compile_ctx cmp c) (compile_sort cmp t1) (compile_sort cmp t2).
+Proof.
+  induction 2;
+    basic_goal_prep; try use_rule_in_wf;
+      basic_core_firstorder_crush.
+  (*TODO: why is this needed? should be automated*)
+  all: use_rule_in_wf;autorewrite with lang_core utils in *;
+    intuition eauto with lang_core.
+Qed.
+
+
+Lemma inductive_implies_semantic_term_axiom ls lt cmp name c e1 e2 t
+  : wf_lang lt -> preserving_compiler_ext [] lt cmp ls -> wf_lang ls ->
+    In (name, term_eq_rule c e1 e2 t) ls ->
+    eq_term lt (compile_ctx cmp c) (compile_sort cmp t) (compile cmp e1) (compile cmp e2).
+Proof.
+  induction 2;
+    basic_goal_prep;
+    try use_rule_in_wf;
+    basic_core_firstorder_crush.
+  (*TODO: why is this needed? should be automated*)
+  all: use_rule_in_wf;autorewrite with lang_core utils in *;
+    intuition eauto with lang_core.
+Qed.
+
+
+Lemma with_names_from_compile_ctx (A:Type) cmp c (s : list A)
+  : with_names_from (compile_ctx cmp c) s
+    = with_names_from c s.
+Proof.
+  revert s; induction c;
+    destruct s; break; basic_core_crush.
+  cbn.
+  f_equal; basic_core_crush.
+Qed.
+  
+
+
+
+Lemma compile_id_args A cmp (c : named_list A)
+  : map (compile cmp) (id_args c) = id_args c.
+Proof.
+  unfold id_args.
+  induction c; 
+    basic_goal_prep;
+    basic_core_crush.
+Qed.
+Hint Rewrite compile_id_args : lang_core.
+
+Lemma fst_equal_id_args_equal A B (c1 : named_list A) (c2 : named_list B)
+  : map fst c1 = map fst c2 -> id_args c1 = id_args c2.
+Proof.
+  unfold id_args; basic_core_crush.
+Qed.
+
+Lemma compile_ctx_fst_equal cmp c
+  : map fst (compile_ctx cmp c) = map fst c.
+Proof.
+  induction c; break; simpl; f_equal; auto.
+Qed.
+ 
+
+Lemma inductive_implies_semantic_sort_rule_id ls lt cmp name c args
+  : wf_lang lt -> preserving_compiler_ext [] lt cmp ls -> wf_lang ls ->
+    In (name, sort_rule c args) ls ->
+    wf_sort lt (compile_ctx cmp c) (compile_sort cmp (scon name (id_args c))).
+Proof.
+  intros wfl pr wfl';
+    revert wfl'; induction pr;
+      basic_goal_prep;
+      with_rule_in_wf_crush.
+  all: try eapply all_constructors_ctx_from_wf; eauto with lang_core.
+  {
+    my_case Hname (eqb name n);[|case_match]; basic_core_firstorder_crush.
+  }
+  {
+    use_rule_in_wf; basic_core_crush.
+  }
+  {
+    my_case Hname (eqb name n);[|case_match]; basic_core_crush.
+  }
+  4:{
+    use_rule_in_wf; basic_core_crush.
+  }
+  (*TODO: eqb? where did this come from?*)
+  all: constructor.
+Qed.
+
+
+
+Lemma inductive_implies_semantic_term_rule_id ls lt cmp name c args t
+  : wf_lang lt -> preserving_compiler_ext [] lt cmp ls -> wf_lang ls ->
+    In (name, term_rule c args t) ls ->
+    wf_term lt (compile_ctx cmp c) (compile cmp (con name (id_args c))) (compile_sort cmp t).
+Proof.
+  intros wfl pr wfl';
+    revert wfl'; induction pr;
+      basic_goal_prep;
+      try use_rule_in_wf;
+      basic_core_firstorder_crush.
+  all: try solve [use_rule_in_wf; basic_core_crush].
+  {
+    my_case Hname (eqb name n);[|case_match]; basic_core_crush.
+  }
+  {
+    my_case Hname (eqb name n);[|case_match]; basic_core_crush.
+  }
+Qed.
+
+
+
+Lemma lookup_in_dom s n
+  : In n (map fst s) -> In (subst_lookup s n) (map snd s).
+Proof.
+  induction s;
+    basic_goal_prep;
+    basic_core_crush.
+  case_match; basic_core_crush.
+Qed.
+
+(*
+Lemma wf_con_id_args_subst' A (c : named_list A) s
+  : forall n e, In n (map fst c) ->
+                In n (map fst s) ->
+                In e (id_args c)[/s/] -> In e (map snd s).
+Proof.
+  induction c;
+    basic_goal_prep;
+    basic_core_crush.
+  (apply lookup_in_dom; assumption).
+  
+  
+  rewrite IHc.
+  unfold args_subst.
+*)
+
+
+Lemma compile_subst_lookup cmp s n
+  : compile cmp (subst_lookup s n)
+  = subst_lookup (compile_subst cmp s) n.
+Proof.
+  induction s;
+    basic_goal_prep;
+    basic_core_crush.
+  case_match; basic_core_crush.
+Qed.
+Hint Rewrite compile_subst_lookup : lang_core.
+
+
+Lemma combine_subst args l s
+  : (combine args l)[/s/] = combine args l[/s/].
+Proof.
+  revert args.
+  induction l;
+    destruct args;
+    basic_goal_prep;
+    basic_core_crush.
+Qed.
+
+
+Lemma lang_compiler_sort_case_args_eq cmp_pre lt cmp ls n c args args' e
+  : preserving_compiler_ext cmp_pre lt cmp ls ->
+    all_fresh ls ->
+    In (n, sort_rule c args) ls ->
+    In (n, sort_case args' e) cmp ->
+    args' = map fst c.
+Proof.
+  induction 1; basic_goal_prep; basic_core_crush.
+  match goal with
+    [Hp : preserving_compiler_ext _ _ _ _,
+          H : fresh _ _|-_]=>
+    pose proof (fresh_lang_fresh_cmp Hp H)
+  end.
+  basic_core_crush.
+Qed.
+Hint Resolve lang_compiler_sort_case_args_eq : lang_core.
+
+Lemma lang_compiler_term_case_args_eq cmp_pre lt cmp ls n c args args' e t
+  : preserving_compiler_ext cmp_pre lt cmp ls ->
+    all_fresh ls ->
+    In (n, term_rule c args t) ls ->
+    In (n, term_case args' e) cmp ->
+    args' = map fst c.
+Proof.
+  (*TODO: takes a long time*)
+  induction 1; basic_goal_prep; basic_core_firstorder_crush.
+  match goal with
+    [Hp : preserving_compiler_ext _ _ _ _,
+          H : fresh _ _|-_]=>
+    pose proof (fresh_lang_fresh_cmp Hp H)
+  end.
+  basic_core_crush.
+Qed.
+Hint Resolve lang_compiler_term_case_args_eq : lang_core.
+
+
+Lemma sort_case_in_preserving_well_scoped cmp_pre tgt cmp src n args t
+  : preserving_compiler_ext cmp_pre tgt cmp src ->
+    ws_lang tgt ->
+    In (n, sort_case args t) cmp ->
+    well_scoped args t.
+Proof.
+  induction 1; basic_goal_prep; basic_core_firstorder_crush.
+  erewrite <- compile_ctx_fst_equal.
+  eapply wf_sort_implies_ws; eauto; eauto with term lang_core.
+Qed.
+Hint Resolve sort_case_in_preserving_well_scoped : lang_core.
+
+
+Lemma term_case_in_preserving_well_scoped cmp_pre tgt cmp src n args t
+  : preserving_compiler_ext cmp_pre tgt cmp src ->
+    ws_lang tgt ->
+    In (n, term_case args t) cmp ->
+    well_scoped args t.
+Proof.
+  induction 1; basic_goal_prep; basic_core_firstorder_crush.
+  erewrite <- compile_ctx_fst_equal.
+  eapply wf_term_implies_ws; eauto; eauto with term lang_core.
+Qed.
+Hint Resolve term_case_in_preserving_well_scoped : lang_core.
+
+(*TODO: move to term?
+  TODO: make type inference smoother
+*)
+Lemma subst_term_default s
+  : (@default term (@term_default V _) : term)[/s/]
+    = (@default term (@term_default V _) : term).
+Proof.
+  unfold default.
+  unfold term_default.
+  simpl.
+  reflexivity.
+Qed.
+
+Local Lemma distribute_compile_subst tgt cmp src s
+  : preserving_compiler_ext [] tgt cmp src ->
+    all_fresh src ->
+    ws_lang tgt ->
+    (forall c t,
+        wf_sort src c t ->
+        map fst c = map fst s ->
+        compile_sort cmp t[/s/] = (compile_sort cmp t)[/compile_subst cmp s/])
+    /\ (forall c e t,
+           wf_term src c e t ->
+           map fst c = map fst s ->
+           compile cmp e[/s/] = (compile cmp e)[/compile_subst cmp s/])
+    /\ (forall c s' c',
+           wf_args src c s' c' ->
+           map fst c = map fst s ->
+           compile_args cmp s'[/s/] = (compile_args cmp s')[/compile_subst cmp s/]).
+Proof using.
+  intros; apply wf_judge_ind; 
+    basic_goal_prep;
+    basic_core_crush.
+  {
+    case_match; basic_core_crush.
+    case_match; basic_core_firstorder_crush;
+      pose proof (lang_compiler_sort_case_args_eq _ _ _ _ _ H H0 H2 HeqH4);
+      basic_core_firstorder_crush.
+    {
+      fold_Substable.
+      match goal with
+        [H : compile_args _ _ = _|-_] =>
+        unfold compile_args in H;
+          rewrite H
+      end.
+      erewrite with_names_from_args_subst.
+      reflexivity.
+    }
+  }
+  {
+    case_match; basic_core_crush.
+    case_match; basic_core_firstorder_crush.
+    pose proof (lang_compiler_term_case_args_eq _ _ _ _ _ _ H H0 H2 HeqH4);
+      basic_core_firstorder_crush.
+    {
+      fold_Substable.
+      match goal with
+        [H : compile_args _ _ = _|-_] =>
+        unfold compile_args in H;
+          rewrite H
+      end.
+      erewrite with_names_from_args_subst.
+      reflexivity.
+    }
+    pose proof (lang_compiler_term_case_args_eq _ _ _ _ _ _ H H0 H2 HeqH4);
+      basic_core_firstorder_crush.
+  }
+Qed.
+
+Lemma compile_term_subst tgt cmp src s c e t
+  : preserving_compiler_ext [] tgt cmp src ->
+    all_fresh src ->
+    ws_lang tgt ->
+    wf_term src c e t ->
+    map fst c = map fst s ->
+    compile cmp e[/s/] = (compile cmp e)[/compile_subst cmp s/].
+Proof.
+  intros; eapply distribute_compile_subst; eassumption.
+Qed.
+Hint Rewrite compile_term_subst : lang_core.
+
+
+Lemma compile_sort_subst tgt cmp src s c t
+  : preserving_compiler_ext [] tgt cmp src ->
+    all_fresh src ->
+    ws_lang tgt ->
+    wf_sort src c t ->
+    map fst c = map fst s ->
+    compile_sort cmp t[/s/] = (compile_sort cmp t)[/compile_subst cmp s/].
+Proof.
+  intros; eapply distribute_compile_subst; eassumption.
+Qed.
+Hint Rewrite compile_sort_subst : lang_core.
+
+
+Lemma compile_args_subst tgt cmp src s c s' c'
+  : preserving_compiler_ext [] tgt cmp src ->
+    all_fresh src ->
+    ws_lang tgt ->
+    wf_args src c s' c' ->
+    map fst c = map fst s ->
+    compile_args cmp s'[/s/] = (compile_args cmp s')[/compile_subst cmp s/].
+Proof.
+  intros; eapply distribute_compile_subst; eassumption.
+Qed.
+Hint Rewrite compile_args_subst : lang_core.
+
+Lemma compile_subst_with_names_from A cmp (c':named_list A) s
+  : (compile_subst cmp (with_names_from c' s)) = with_names_from c' (map (compile cmp) s).
+Proof.
+  unfold compile_subst.
+  rewrite <- with_names_from_map_is_named_map.
+  reflexivity.
+Qed.
+
+Lemma compile_scon cmp args s name t
+  : all_fresh cmp ->
+    In (name, sort_case args t) cmp ->
+    (compile_sort cmp (scon name s)) = t[/(combine args (compile_args cmp s))/].
+Proof.
+  basic_goal_prep; repeat case_match; basic_core_crush.
+  {
+    (*TODO: should be automated; how best to do so?*)
+    pose proof (in_all_fresh_same _ _ _ _ H H0 HeqH1).
+    basic_core_crush.
+  }
+  {
+    (*TODO: should be automated; how best to do so?*)
+    pose proof (in_all_fresh_same _ _ _ _ H H0 HeqH1).
+    basic_core_crush.
+  }
+  {
+    exfalso.
+    (*TODO: why isn't this automated already?*)
+    eapply named_list_lookup_none; eauto.
+  }
+Qed.
+  
+Lemma lang_compiler_conflict_sort_term cmp_pre lt cmp ls n c args args' e
+  : preserving_compiler_ext cmp_pre lt cmp ls ->
+    all_fresh ls ->
+    In (n, sort_rule c args) ls ->
+    In (n, term_case args' e) cmp ->
+    False.
+Proof.
+  induction 1; basic_goal_prep; basic_core_crush.
+  match goal with
+    [Hp : preserving_compiler_ext _ _ _ _,
+          H : fresh _ _|-_]=>
+    pose proof (fresh_lang_fresh_cmp Hp H)
+  end.
+  basic_core_crush.
+Qed.
+Hint Resolve lang_compiler_conflict_sort_term : lang_core.
+
+  
+Lemma lang_compiler_conflict_term_sort cmp_pre lt cmp ls n c args args' e t
+  : preserving_compiler_ext cmp_pre lt cmp ls ->
+    all_fresh ls ->
+    In (n, term_rule c args t) ls ->
+    In (n, sort_case args' e) cmp ->
+    False.
+Proof.
+  induction 1; basic_goal_prep; basic_core_firstorder_crush.
+  match goal with
+    [Hp : preserving_compiler_ext _ _ _ _,
+          H : fresh _ _|-_]=>
+    pose proof (fresh_lang_fresh_cmp Hp H)
+  end.
+  eauto with utils.
+Qed.
+Hint Resolve lang_compiler_conflict_term_sort : lang_core.
+  
+  
+(*TODO: do the same thing for terms*)
+Lemma inductive_implies_semantic_sort_rule ls lt cmp name c c' args s
+  : wf_lang lt -> preserving_compiler_ext [] lt cmp ls -> wf_lang ls ->
+    In (name, sort_rule c' args) ls ->
+    wf_ctx lt (compile_ctx cmp c') ->
+    wf_args lt (compile_ctx cmp c) (compile_args cmp s) (compile_ctx cmp c') ->
+    wf_sort lt (compile_ctx cmp c) (compile_sort cmp (scon name s)).
+Proof.
+  intros.
+  replace (scon name s) with (scon name (id_args c'))[/(with_names_from c' s)/].
+  erewrite compile_sort_subst; try eassumption; eauto with lang_core.
+  2:{
+    econstructor; [eassumption |].
+    basic_core_crush.
+  }
+  eapply wf_sort_subst_monotonicity; auto.
+  {
+    eapply inductive_implies_semantic_sort_rule_id; eauto.
+  }
+  all: basic_core_firstorder_crush.
+  {
+    rewrite compile_subst_with_names_from.
+    erewrite <- with_names_from_compile_ctx.
+    eapply wf_subst_from_wf_args; basic_core_crush.
+  }
+  {
+    pose proof (wf_args_length_eq H4).
+    unfold compile_args in H5.
+    unfold compile_ctx in H5.
+    basic_core_crush.
+  }
+  {
+    simpl; f_equal.
+    rewrite wf_con_id_args_subst; basic_core_firstorder_crush.
+    rewrite <- all_fresh_compile_ctx.
+    eauto with lang_core.
+    pose proof (wf_args_length_eq H4).
+    unfold compile_args in H5.
+    unfold compile_ctx in H5.
+    basic_core_crush.
+  }
+Qed.
+
+Lemma inductive_implies_semantic_term_rule ls lt cmp name c c' args t s
+  : wf_lang lt -> preserving_compiler_ext [] lt cmp ls -> wf_lang ls ->
+    In (name, term_rule c' args t) ls ->
+    wf_ctx lt (compile_ctx cmp c') ->
+    wf_args lt (compile_ctx cmp c) (compile_args cmp s) (compile_ctx cmp c') ->
+    wf_term lt (compile_ctx cmp c) (compile cmp (con name s)) (compile_sort cmp t)[/compile_subst cmp (with_names_from c' s)/].
+Proof.
+  intros.
+  replace (con name s) with (con name (id_args c'))[/(with_names_from c' s)/].
+  erewrite compile_term_subst; try eassumption; eauto with lang_core.
+  2:{
+    econstructor; [eassumption |].
+    basic_core_crush.
+  }
+  eapply wf_term_subst_monotonicity; auto.
+  {
+    eapply inductive_implies_semantic_term_rule_id; eauto.
+  }
+  {
+    basic_core_crush.
+  }
+  {
+    rewrite compile_subst_with_names_from.
+    erewrite <- with_names_from_compile_ctx.
+    eapply wf_subst_from_wf_args; basic_core_crush.
+  }
+  {
+    pose proof (wf_args_length_eq H4).
+    unfold compile_args in H5.
+    unfold compile_ctx in H5.
+    basic_core_firstorder_crush.
+  }
+  {
+    simpl; f_equal.
+    fold_Substable.
+    rewrite wf_con_id_args_subst; basic_core_firstorder_crush.
+    rewrite <- all_fresh_compile_ctx.
+    eauto with lang_core.
+    pose proof (wf_args_length_eq H4).
+    unfold compile_args in H5.
+    unfold compile_ctx in H5.
+    basic_core_crush.
+  }
+Qed.
+
+
+(*TODO: maybe not necessary with better strengthening lemma?
+  See what happens when I use the better one
+*)
+Variant rule_compiles_with {lt cmp} : rule -> Prop :=
+| sort_rule_compiles_with c args
+  : wf_ctx lt (compile_ctx cmp c) -> rule_compiles_with (sort_rule c args)
+| term_rule_compiles_with c args t
+  : wf_ctx lt (compile_ctx cmp c) ->
+    wf_sort lt (compile_ctx cmp c) (compile_sort cmp t) ->
+    rule_compiles_with (term_rule c args t)
+(*Similar properties are not necessary for eq rules*)
+| sort_eq_rule_compiles_with c t1 t2 : rule_compiles_with (sort_eq_rule c t1 t2)
+| term_eq_rule_compiles_with c e1 e2 t : rule_compiles_with (term_eq_rule c e1 e2 t).
+Arguments rule_compiles_with : clear implicits.
+                       
+Definition lang_compiles_with lt cmp : lang -> Prop :=
+  all (fun p => rule_compiles_with lt cmp (snd p)).
+
+
+Lemma lang_compiles_with_sort_ctx_in lt cmp ls n c' args
+  : lang_compiles_with lt cmp ls ->
+    In (n, sort_rule c' args) ls ->
+    wf_ctx lt (compile_ctx cmp c').
+Proof.
+  induction ls; 
+    basic_goal_prep;
+    basic_core_firstorder_crush.
+  (*TODO: This could be automated w/ an inversion lemma*)
+  match goal with
+    [H : rule_compiles_with _ _ _ |-_]=>
+    inversion H; basic_core_crush
+  end.
+Qed.
+Local Hint Resolve lang_compiles_with_sort_ctx_in : lang_core.
+
+Lemma lang_compiles_with_term_ctx_in lt cmp ls n c' args t
+  : lang_compiles_with lt cmp ls ->
+    In (n, term_rule c' args t) ls ->
+    wf_ctx lt (compile_ctx cmp c').
+Proof.
+  induction ls; 
+    basic_goal_prep;
+    basic_core_firstorder_crush.
+  (*TODO: This could be automated w/ an inversion lemma*)
+  match goal with
+    [H : rule_compiles_with _ _ _ |-_]=>
+    inversion H; basic_core_crush
+  end.
+Qed.
+Local Hint Resolve lang_compiles_with_term_ctx_in : lang_core.
+
+Lemma lang_compiles_with_term_sort_in lt cmp ls n c' args t
+  : lang_compiles_with lt cmp ls ->
+    In (n, term_rule c' args t) ls ->
+    wf_sort lt (compile_ctx cmp c') (compile_sort cmp t).
+Proof.
+  induction ls; 
+    basic_goal_prep;
+    basic_core_firstorder_crush.
+  (*TODO: This could be automated w/ an inversion lemma*)
+  match goal with
+    [H : rule_compiles_with _ _ _ |-_]=>
+    inversion H; basic_core_crush
+  end.
+Qed.
+Local Hint Resolve lang_compiles_with_term_sort_in : lang_core.
+
+
+Local Lemma inductive_implies_semantic' lt cmp ls
+  : wf_lang ls ->
+    wf_lang lt ->
+    preserving_compiler_ext [] lt cmp ls ->
+    lang_compiles_with lt cmp ls ->
+    semantics_preserving lt cmp ls.
+Proof.
+  intros; apply judge_ind; 
+    basic_goal_prep;
+    basic_core_firstorder_crush.
+  {
+    eapply inductive_implies_semantic_sort_axiom; eassumption.
+  }
+  {
+    erewrite !compile_sort_subst.
+    all: try match goal with
+               [|- map fst _ = map fst _] =>
+               symmetry; eauto with lang_core
+             end.
+    all: basic_core_firstorder_crush.
+  }
+  {
+    erewrite !compile_sort_subst.
+    erewrite !compile_term_subst.
+    all: try match goal with
+               [|- map fst _ = map fst _] =>
+               symmetry; eauto with lang_core
+             end.
+    all: basic_core_firstorder_crush.
+  }
+  {
+    eapply inductive_implies_semantic_term_axiom; eassumption.
+  }
+  {
+    constructor; basic_core_firstorder_crush.
+    match goal with
+      [ H : eq_term _ _ (compile_sort _ _) _ _|-_] =>
+      erewrite !compile_sort_subst in H
+    end.
+    all: try match goal with
+               [|- map fst _ = map fst _] =>
+               symmetry; eauto with lang_core
+             end.
+    all: basic_core_firstorder_crush.
+  }
+  {
+    eapply inductive_implies_semantic_sort_rule; try eassumption.
+    all: try use_rule_in_wf; basic_core_firstorder_crush.
+  }
+  {
+    erewrite compile_sort_subst; eauto.
+    all: try match goal with
+               [|- map fst _ = map fst _] =>
+               symmetry; eauto with lang_core
+             end.
+    all: basic_core_firstorder_crush.
+    assert (wf_ctx ls c') by (use_rule_in_wf; basic_core_crush).
+    eapply inductive_implies_semantic_term_rule; try (auto;eassumption).
+    all: try use_rule_in_wf; basic_core_firstorder_crush.
+  }
+  {
+    constructor.
+    apply in_named_map; assumption.
+  }
+  {
+    constructor; basic_core_firstorder_crush.
+    match goal with
+      [ H : wf_term _ _ _ (compile_sort _ _) |-_] =>
+      erewrite !compile_sort_subst in H
+    end.
+    all: try match goal with
+               [|- map fst _ = map fst _] =>
+               symmetry; eauto with lang_core
+             end.
+    all: basic_core_firstorder_crush.
+    match goal with
+      [H : context [compile_subst _ (with_names_from _ _)]|-_] =>
+      rewrite compile_subst_with_names_from in H
+    end.
+    rewrite with_names_from_compile_ctx.
+    assumption.
+  }
+Qed.
+
+Local Lemma inductive_implies_semantic_ctx' lt cmp ls
+  : wf_lang ls ->
+    wf_lang lt ->
+    preserving_compiler_ext [] lt cmp ls ->
+    lang_compiles_with lt cmp ls ->
+    forall c : ctx, wf_ctx ls c -> wf_ctx lt (compile_ctx cmp c).
+Proof.
+  intros wfs wft pc lcw.
+  apply inductive_implies_semantic'; eauto.
+Qed.
+Local Hint Resolve inductive_implies_semantic_ctx' : lang_core.
+
+
+Local Hint Constructors rule_compiles_with : lang_core.
+
+Definition all_constructors_rule P r :=
+  match r with
+  | sort_rule c _ => all (fun '(_, t) => all_constructors_sort P t) c
+  | term_rule c _ t =>
+    (all (fun '(_, t) => all_constructors_sort P t) c)
+    /\ (all_constructors_sort P t)
+  | _ => True
+  end.
+
+Local Lemma rule_compiles_extend_fresh lt cmp r n cc
+  : rule_compiles_with lt cmp r ->
+    all_constructors_rule (fun n0 : V => In n0 (map fst cmp)) r ->
+    fresh n cmp ->
+    all_fresh cmp ->
+    rule_compiles_with lt ((n,cc)::cmp) r.
+Proof.
+  inversion 1; basic_goal_prep; with_rule_in_wf_crush.
+  all: constructor.
+  all: try erewrite compile_strengthen_ctx; eauto.
+  all: try rewrite compile_strengthen_sort; eauto.
+Qed. 
+  
+Local Lemma lang_compiles_extend_fresh lt cmp ls n cc
+  : lang_compiles_with lt cmp ls ->
+    all (fun '(_,r) => all_constructors_rule (fun n0 : V => In n0 (map fst cmp)) r) ls ->
+    fresh n cmp ->
+    all_fresh cmp ->
+    lang_compiles_with lt ((n,cc)::cmp) ls.
+Proof.
+  unfold lang_compiles_with.
+  induction ls; basic_goal_prep; with_rule_in_wf_crush.
+  eapply rule_compiles_extend_fresh; eauto.
+Qed.  
+
+(*TODO: move to core with like lemmas above*)
+Lemma all_constructors_rule_from_wf tgt cmp src r
+  : preserving_compiler_ext [] tgt cmp src ->
+    wf_rule src r ->
+    all_constructors_rule (fun n0 : V => In n0 (map fst cmp)) r.
+Proof.
+  inversion 2; basic_goal_prep;
+    with_rule_in_wf_crush.
+  (*TODO: automation; need to restrict simplify?*)
+  all: eapply all_constructors_ctx_from_wf; eauto.
+Qed.
+Hint Resolve all_constructors_rule_from_wf : lang_core.
+
+Lemma all_constructors_term_weaken (P Q : _ -> Prop) e
+  : (forall n, P n -> Q n) ->
+    all_constructors P e ->
+    all_constructors Q e.
+Proof.
+  intro.
+  induction e; basic_goal_prep; basic_core_firstorder_crush.
+
+  revert dependent l;
+    induction l; basic_goal_prep; basic_core_crush.
+Qed.
+Hint Resolve all_constructors_term_weaken : lang_core.
+
+
+Lemma all_constructors_args_weaken (P Q : _ -> Prop) l
+  : (forall n, P n -> Q n) ->
+    all (all_constructors P) l ->
+    all (all_constructors Q) l.
+Proof.
+  intro;
+    revert dependent l;
+    induction l; basic_goal_prep; basic_core_crush.
+Qed.
+Hint Resolve all_constructors_args_weaken : lang_core.
+
+
+Lemma all_constructors_sort_weaken (P Q : _ -> Prop) e
+  : (forall n, P n -> Q n) ->
+    all_constructors_sort P e ->
+    all_constructors_sort Q e.
+Proof.
+  intro.
+  destruct e; basic_goal_prep; basic_core_crush.
+Qed.
+Hint Resolve all_constructors_sort_weaken : lang_core.
+
+Lemma all_constructors_ctx_weaken (P Q : _ -> Prop) (c : ctx)
+  : (forall n, P n -> Q n) ->
+    all_constructors_ctx P c ->
+    all_constructors_ctx Q c.
+Proof.
+  intro;
+    induction c; basic_goal_prep; basic_core_crush.
+Qed.
+Hint Resolve all_constructors_ctx_weaken : lang_core.
+
+
+Lemma all_constructors_rule_weaken (P Q : _ -> Prop) r
+  : (forall n, P n -> Q n) ->
+    all_constructors_rule P r ->
+    all_constructors_rule Q r.
+Proof.
+  intro;
+    destruct r; basic_goal_prep; basic_core_crush.
+  all: eapply all_constructors_ctx_weaken; eauto.
+Qed.
+Hint Resolve all_constructors_rule_weaken : lang_core.
+
+
+Lemma all_constructors_lang_weaken (P Q : _ -> Prop) (l : lang)
+  : (forall n, P n -> Q n) ->
+    all (fun '(_, t) => all_constructors_rule P t) l ->
+    all (fun '(_, t) => all_constructors_rule Q t) l.
+Proof.
+  intro;
+    induction l; basic_goal_prep; basic_core_crush.
+Qed.
+Hint Resolve all_constructors_lang_weaken : lang_core.
+
+Lemma wf_lang_implies_all_constructors lt l
+  : wf_lang l ->
+    forall cmp,
+    preserving_compiler_ext [] lt cmp l ->
+    all (fun '(_,r) => all_constructors_rule (fun n0 : V => In n0 (map fst cmp)) r) l.
+Proof.
+  induction 1; basic_goal_prep;
+    with_rule_in_wf_crush.
+  (*TODO: break down cmp*)
+  inversion H2; subst.
+  1,2:specialize (IHwf_lang_ext cmp0).
+  3,4:specialize (IHwf_lang_ext cmp).
+  all:eapply all_constructors_lang_weaken.
+  all: try apply IHwf_lang_ext; auto.
+  all:basic_goal_prep; basic_core_firstorder_crush.
+Qed.
+
+
+Local Lemma preserving_compiler_to_lang_compiles_with lt ls
+  : wf_lang ls ->
+    wf_lang lt ->
+    forall cmp,
+    preserving_compiler_ext [] lt cmp ls ->
+    lang_compiles_with lt cmp ls.
+Proof.
+  induction 1; inversion 2; basic_goal_prep; with_rule_in_wf_crush.
+  all: try constructor.
+  all: try rewrite compile_strengthen_ctx; eauto.
+  all: try rewrite compile_strengthen_sort; eauto.
+  all: try apply lang_compiles_extend_fresh; eauto with lang_core.
+  all: try eapply wf_lang_implies_all_constructors; eauto.
+  all: eapply all_constructors_ctx_from_wf; [| eauto..]; eauto.
+Qed.
+
+
+Theorem inductive_implies_semantic lt cmp ls
+  : wf_lang ls ->
+    wf_lang lt ->
+    preserving_compiler_ext [] lt cmp ls ->
+    semantics_preserving lt cmp ls.
+Proof.
+  intros; apply inductive_implies_semantic';
+    eauto using  preserving_compiler_to_lang_compiles_with.
+Qed.
+
+End WithVar.
+
+
+#[export] Hint Rewrite fresh_compile_ctx : lang_core.
+#[export] Hint Rewrite all_fresh_compile_ctx : lang_core.
+#[export] Hint Resolve fresh_lang_fresh_cmp : lang_core.
+#[export] Hint Resolve all_fresh_compiler : lang_core.
+
+#[export] Hint Rewrite compile_strengthen_term : lang_core.
+#[export] Hint Rewrite compile_strengthen_args : lang_core.
+#[export] Hint Rewrite compile_strengthen_sort : lang_core.
+#[export] Hint Rewrite compile_strengthen_ctx : lang_core.
+
+
+#[export] Hint Resolve all_constructors_sort_from_wf : lang_core.
+#[export] Hint Resolve all_constructors_term_from_wf : lang_core.
+#[export] Hint Resolve all_constructors_args_from_wf : lang_core.
+#[export] Hint Resolve all_constructors_ctx_from_wf : lang_core.
+#[export] Hint Rewrite compile_id_args : lang_core.
+#[export] Hint Rewrite compile_subst_lookup : lang_core.
+
+#[export] Hint Resolve lang_compiler_sort_case_args_eq : lang_core.
+#[export] Hint Resolve lang_compiler_term_case_args_eq : lang_core.
+#[export] Hint Resolve sort_case_in_preserving_well_scoped : lang_core.
+#[export] Hint Resolve term_case_in_preserving_well_scoped : lang_core.
+
+#[export] Hint Rewrite compile_term_subst : lang_core.
+#[export] Hint Rewrite compile_sort_subst : lang_core.
+#[export] Hint Rewrite compile_args_subst : lang_core.
+
+#[export] Hint Resolve lang_compiler_conflict_sort_term : lang_core.
+#[export] Hint Resolve lang_compiler_conflict_term_sort : lang_core.
+
+
+#[export] Hint Resolve all_constructors_rule_from_wf : lang_core.
+#[export] Hint Resolve all_constructors_term_weaken : lang_core.
+#[export] Hint Resolve all_constructors_args_weaken : lang_core.
+#[export] Hint Resolve all_constructors_sort_weaken : lang_core.
+#[export] Hint Resolve all_constructors_ctx_weaken : lang_core.
+#[export] Hint Resolve all_constructors_rule_weaken : lang_core.
+#[export] Hint Resolve all_constructors_lang_weaken : lang_core.
